pcuic/theories/PCUICArities.v
@@ -7,7 +7,8 @@ From MetaCoq.PCUIC Require Import PCUICAst PCUICAstUtils PCUICInduction
      PCUICInversion PCUICCumulativity PCUICReduction
      PCUICConfluence PCUICConversion PCUICContextConversion
      PCUICWeakeningEnv PCUICClosed PCUICSubstitution PCUICWfUniverses
-     PCUICWeakening PCUICGeneration PCUICUtils PCUICContexts.
+     PCUICWeakening PCUICGeneration PCUICUtils PCUICContexts
+     PCUICWellScopedCumulativity.
 
 From Equations Require Import Equations.
 Require Import Equations.Prop.DepElim.
@@ -28,6 +29,9 @@ Proof.
   eexists; econstructor; eauto.
 Qed.
 
+Definition wf_typing_spine {cf} {Σ Γ T args T'} :=
+  isType Σ Γ T × typing_spine Σ Γ T args T'.
+
 Hint Resolve @isType_Sort : pcuic.
 
 Lemma isArity_it_mkProd_or_LetIn Γ t : isArity t -> isArity (it_mkProd_or_LetIn Γ t).
@@ -37,608 +41,609 @@ Proof.
   destruct x as [? [?|] ?]; simpl; auto.
 Qed.
 
-Lemma invert_cumul_arity_l {cf:checker_flags} Σ (Γ : context) (C : term) T :
-  wf Σ.1 ->
-  Σ;;; Γ |- C <= T ->
-  match destArity [] C with
-  | Some (ctx, s) =>
-    ∑ T' ctx' s', red Σ.1 Γ T T' * (destArity [] T' = Some (ctx', s')) * 
-       conv_context Σ (Γ ,,, smash_context [] ctx) (Γ ,,, ctx') * 
-       leq_universe (global_ext_constraints Σ) s s'
-  | None => unit
-  end.
-Proof.
-  intros wfΣ CT.
-  generalize (destArity_spec [] C). destruct destArity as [[ctx p]|].
-  simpl. intros ->. 2:intros _; exact tt.
-  revert Γ T CT.
-  generalize (@le_n #|ctx|).
-  generalize (#|ctx|) at 2. intros n; revert ctx.
-  induction n; intros ctx Hlen Γ T HT.
-  - destruct ctx; simpl in Hlen; try lia.
-    eapply invert_cumul_sort_l in HT as [u' [redT leqT]].
-    exists (tSort u'), [], u'; intuition auto.
-    reflexivity.
-  - destruct ctx using rev_ind.
-    * eapply invert_cumul_sort_l in HT as [u' [redT leqT]].
-      exists (tSort u'), [], u'; intuition auto.  
-      reflexivity.
-    * rewrite it_mkProd_or_LetIn_app in HT; simpl in HT.
-      destruct x as [na [b|] ty]; unfold mkProd_or_LetIn in HT; simpl in *.
-      + eapply invert_cumul_letin_l in HT; auto.
-        unfold subst1 in HT; rewrite subst_it_mkProd_or_LetIn in HT.
-        rewrite app_length /= Nat.add_1_r in Hlen.
-        simpl in HT. specialize (IHn (subst_context [b] 0 ctx) ltac:(rewrite
-        subst_context_length; lia) Γ T HT).
-        destruct IHn as [T' [ctx' [s' [[[redT destT] convctx] leq]]]].
-        clear IHctx.
-        exists T', ctx', s'. intuition auto.
-        rewrite smash_context_app. simpl.
-        now rewrite -smash_context_subst_empty.
-      + eapply invert_cumul_prod_l in HT; auto. 
-        rewrite -> app_length in Hlen.
-        rewrite Nat.add_1_r in Hlen.
-        destruct HT as [na' [A' [B' [[redT convT] HT]]]].
-        specialize (IHn ctx ltac:(lia) (Γ ,, vass na' A') B').
-        forward IHn. eapply cumul_conv_ctx; eauto.
-        constructor; pcuic. clear IHctx.
-        destruct IHn as [T' [ctx' [s' [[[redT' destT] convctx] leq]]]].
-        exists (tProd na' A' T'), (ctx' ++ [vass na' A']), s'. intuition auto. 2:simpl.
-        -- transitivity (tProd na' A' B'); auto.
-          eapply red_prod. reflexivity. apply redT'.
-        -- now rewrite destArity_app destT.
-        -- rewrite smash_context_app /= .
-          rewrite !app_context_assoc.
-          assert (#|smash_context [] ctx| = #|ctx'|).
-          { apply All2_fold_length in convctx.
-            autorewrite with len in convctx |- *.
-            simpl in convctx. simpl. lia. }
-          eapply All2_fold_app; auto.
-          apply All2_fold_app_inv in convctx; auto.
-          constructor; pcuic. constructor; auto.
-          eapply All2_fold_app_inv in convctx as [_ convctx].
-          unshelve eapply (All2_fold_impl convctx).
-          simpl; pcuicfo. destruct X. constructor; auto.
-          eapply conv_conv_ctx; eauto.
-          eapply All2_fold_app. constructor; pcuic.
-          constructor; pcuic. constructor; pcuic. now symmetry.
-          apply All2_fold_refl. intros.
-          destruct x as [na'' [b'|] ty']; constructor; reflexivity.
-          constructor; pcuic. 
-          eapply conv_conv_ctx; eauto.
-          eapply All2_fold_app. constructor; pcuic.
-          constructor; pcuic. constructor; pcuic. now symmetry.
-          apply All2_fold_refl. intros.
-          destruct x as [na'' [b''|] ty']; constructor; reflexivity.
-          eapply conv_conv_ctx; eauto.
-          eapply All2_fold_app. constructor; pcuic.
-          constructor; pcuic. constructor; pcuic. now symmetry.
-          apply All2_fold_refl. intros.
-          destruct x as [? [?|] ?]; constructor; reflexivity.
-          auto.
-Qed.
+Section WfEnv.
+  Context {cf:checker_flags} {Σ : global_env_ext} {wfΣ : wf Σ}.
 
-Lemma isType_tProd {cf:checker_flags} {Σ : global_env_ext} (HΣ' : wf Σ)
-      {Γ} {na A B}
-  : isType Σ Γ (tProd na A B)
-    <~> (isType Σ Γ A × isType Σ (Γ,, vass na A) B).
-Proof.
-  split; intro HH.
-  - destruct HH as [s H].
-    apply inversion_Prod in H; tas. destruct H as [s1 [s2 [HA [HB Hs]]]].
-    split.
-    * eexists; tea.
-    * eexists; tea.
-  - destruct HH as [HA HB].
-    destruct HA as [sA HA], HB as [sB HB].
-    eexists. econstructor; eassumption.
-Defined.
+  Lemma invert_cumul_arity_l (Γ : context) (C : term) T :
+    Σ;;; Γ ⊢ C ≤ T ->
+    match destArity [] C with
+    | Some (ctx, s) =>
+      ∑ T' ctx' s',
+        [× Σ ;;; Γ ⊢ T ⇝ T', (destArity [] T' = Some (ctx', s')),
+          closed_conv_context Σ (Γ ,,, smash_context [] ctx) (Γ ,,, ctx') &
+          leq_universe (global_ext_constraints Σ) s s']
+    | None => unit
+    end.
+  Proof.
+    intros CT.
+    generalize (destArity_spec [] C). destruct destArity as [[ctx p]|].
+    simpl. intros ->. 2:intros _; exact tt.
+    revert Γ T CT.
+    generalize (@le_n #|ctx|).
+    generalize (#|ctx|) at 2. intros n; revert ctx.
+    induction n; intros ctx Hlen Γ T HT.
+    - destruct ctx; simpl in Hlen; try lia.
+      eapply equality_Sort_l_inv in HT as [u' [redT leqT]].
+      exists (tSort u'), [], u'; split; auto.
+      cbn. eapply closed_context_equality_refl; eauto with fvs.
+    - destruct ctx using rev_ind.
+      * eapply equality_Sort_l_inv in HT as [u' [redT leqT]].
+        exists (tSort u'), [], u'; split; auto; cbn.  
+        apply closed_context_equality_refl; eauto with fvs.
+      * rewrite it_mkProd_or_LetIn_app in HT; simpl in HT.
+        destruct x as [na [b|] ty]; unfold mkProd_or_LetIn in HT; simpl in *.
+        + eapply equality_LetIn_l_inv in HT; auto.
+          unfold subst1 in HT; rewrite subst_it_mkProd_or_LetIn in HT.
+          rewrite app_length /= Nat.add_1_r in Hlen.
+          simpl in HT. specialize (IHn (subst_context [b] 0 ctx) ltac:(rewrite
+          subst_context_length; lia) Γ T HT).
+          destruct IHn as [T' [ctx' [s' [redT destT convctx leq]]]].
+          clear IHctx.
+          exists T', ctx', s'. split; auto.
+          rewrite smash_context_app. simpl.
+          now rewrite -smash_context_subst_empty.
+        + eapply invert_y_prod_l in HT; auto. 
+          rewrite -> app_length in Hlen.
+          rewrite Nat.add_1_r in Hlen.
+          destruct HT as [na' [A' [B' [[redT convT] HT]]]].
+          specialize (IHn ctx ltac:(lia) (Γ ,, vass na' A') B').
+          forward IHn. eapply cumul_conv_ctx; eauto.
+          constructor; pcuic. clear IHctx.
+          destruct IHn as [T' [ctx' [s' [[[redT' destT] convctx] leq]]]].
+          exists (tProd na' A' T'), (ctx' ++ [vass na' A']), s'. intuition auto. 2:simpl.
+          -- transitivity (tProd na' A' B'); auto.
+            eapply red_prod. reflexivity. apply redT'.
+          -- now rewrite destArity_app destT.
+          -- rewrite smash_context_app /= .
+            rewrite !app_context_assoc.
+            assert (#|smash_context [] ctx| = #|ctx'|).
+            { apply All2_fold_length in convctx.
+              autorewrite with len in convctx |- *.
+              simpl in convctx. simpl. lia. }
+            eapply All2_fold_app; auto.
+            apply All2_fold_app_inv in convctx; auto.
+            constructor; pcuic. constructor; auto.
+            eapply All2_fold_app_inv in convctx as [_ convctx].
+            unshelve eapply (All2_fold_impl convctx).
+            simpl; pcuicfo. destruct X. constructor; auto.
+            eapply conv_conv_ctx; eauto.
+            eapply All2_fold_app. constructor; pcuic.
+            constructor; pcuic. constructor; pcuic. now symmetry.
+            apply All2_fold_refl. intros.
+            destruct x as [na'' [b'|] ty']; constructor; reflexivity.
+            constructor; pcuic. 
+            eapply conv_conv_ctx; eauto.
+            eapply All2_fold_app. constructor; pcuic.
+            constructor; pcuic. constructor; pcuic. now symmetry.
+            apply All2_fold_refl. intros.
+            destruct x as [na'' [b''|] ty']; constructor; reflexivity.
+            eapply conv_conv_ctx; eauto.
+            eapply All2_fold_app. constructor; pcuic.
+            constructor; pcuic. constructor; pcuic. now symmetry.
+            apply All2_fold_refl. intros.
+            destruct x as [? [?|] ?]; constructor; reflexivity.
+            auto.
+  Qed.
 
-Lemma isType_subst {cf:checker_flags} {Σ : global_env_ext} (HΣ' : wf Σ)
-      {Γ Δ} (HΓ : wf_local Σ (Γ ,,, Δ)) {A} s :
+  Lemma isType_tProd {cf:checker_flags} {Σ : global_env_ext} (HΣ' : wf Σ)
+        {Γ} {na A B}
+    : isType Σ Γ (tProd na A B)
+      <~> (isType Σ Γ A × isType Σ (Γ,, vass na A) B).
+  Proof.
+    split; intro HH.
+    - destruct HH as [s H].
+      apply inversion_Prod in H; tas. destruct H as [s1 [s2 [HA [HB Hs]]]].
+      split.
+      * eexists; tea.
+      * eexists; tea.
+    - destruct HH as [HA HB].
+      destruct HA as [sA HA], HB as [sB HB].
+      eexists. econstructor; eassumption.
+  Defined.
+
+  Lemma isType_subst {cf:checker_flags} {Σ : global_env_ext} (HΣ' : wf Σ)
+        {Γ Δ} (HΓ : wf_local Σ (Γ ,,, Δ)) {A} s :
+      subslet Σ Γ s Δ ->
+      isType Σ (Γ ,,, Δ) A -> 
+      isType Σ Γ (subst0 s A).
+  Proof.
+    intros sub [u Hu].
+    exists u. eapply (substitution _ _ Δ s [] _ _ HΣ' sub Hu).
+  Qed.
+
+  Lemma isType_subst_gen {cf:checker_flags} {Σ : global_env_ext} (HΣ' : wf Σ) {Γ Δ Δ'} {A} s :
     subslet Σ Γ s Δ ->
-    isType Σ (Γ ,,, Δ) A -> 
-    isType Σ Γ (subst0 s A).
-Proof.
-  intros sub [u Hu].
-  exists u. eapply (substitution _ _ Δ s [] _ _ HΣ' sub Hu).
-Qed.
+    isType Σ (Γ ,,, Δ ,,, Δ') A -> 
+    isType Σ (Γ ,,, subst_context s 0 Δ') (subst s #|Δ'| A).
+  Proof.
+    intros sub [s' Hs].
+    exists s'. eapply (substitution _ _ Δ s _ _ _ HΣ' sub Hs).
+  Qed.
 
-Lemma isType_subst_gen {cf:checker_flags} {Σ : global_env_ext} (HΣ' : wf Σ) {Γ Δ Δ'} {A} s :
-  subslet Σ Γ s Δ ->
-  isType Σ (Γ ,,, Δ ,,, Δ') A -> 
-  isType Σ (Γ ,,, subst_context s 0 Δ') (subst s #|Δ'| A).
-Proof.
-  intros sub [s' Hs].
-  exists s'. eapply (substitution _ _ Δ s _ _ _ HΣ' sub Hs).
-Qed.
+  Lemma isType_apply {cf} {Σ : global_env_ext} {wfΣ : wf Σ} Γ na A B t : 
+    isType Σ Γ (tProd na A B) ->
+    Σ ;;; Γ |- t : A ->
+    isType Σ Γ (B {0 := t}).
+  Proof.
+    move/isType_tProd => [hA hB] ht.
+    eapply (isType_subst _ (Δ:= [vass na A])); tea.
+    constructor; auto. pcuic.
+    now eapply subslet_ass_tip.
+  Qed.
 
-Lemma isType_apply {cf} {Σ : global_env_ext} {wfΣ : wf Σ} Γ na A B t : 
-  isType Σ Γ (tProd na A B) ->
-  Σ ;;; Γ |- t : A ->
-  isType Σ Γ (B {0 := t}).
-Proof.
-  move/isType_tProd => [hA hB] ht.
-  eapply (isType_subst _ (Δ:= [vass na A])); tea.
-  constructor; auto. pcuic.
-  now eapply subslet_ass_tip.
-Qed.
+  Lemma typing_spine_letin_inv {cf:checker_flags} {Σ Γ na b B T args S} : 
+    wf Σ.1 ->
+    typing_spine Σ Γ (tLetIn na b B T) args S ->
+    typing_spine Σ Γ (T {0 := b}) args S.
+  Proof.
+    intros wfΣ Hsp.
+    depelim Hsp.
+    constructor. auto.
+    now eapply equality_LetIn_l_inv in c.
+    econstructor; eauto.
+    now eapply equality_LetIn_l_inv in c.
+  Qed.
 
-Definition wf_typing_spine {cf} {Σ Γ T args T'} :=
-  isType Σ Γ T × typing_spine Σ Γ T args T'.
+  Lemma typing_spine_letin {cf:checker_flags} {Σ Γ na b B T args S} : 
+    wf Σ.1 ->
+    typing_spine Σ Γ (T {0 := b}) args S ->
+    typing_spine Σ Γ (tLetIn na b B T) args S.
+  Proof.
+    intros wfΣ Hsp.
+    depelim Hsp.
+    constructor. auto.
+    etransitivity. eapply red_cumul. eapply red1_red, red_zeta. auto.
+    econstructor; eauto.
+    etransitivity. eapply red_cumul. eapply red1_red, red_zeta. auto.
+  Qed.
 
-Lemma typing_spine_letin_inv {cf:checker_flags} {Σ Γ na b B T args S} : 
-  wf Σ.1 ->
-  typing_spine Σ Γ (tLetIn na b B T) args S ->
-  typing_spine Σ Γ (T {0 := b}) args S.
-Proof.
-  intros wfΣ Hsp.
-  depelim Hsp.
-  constructor. auto.
-  now eapply invert_cumul_letin_l in c.
-  econstructor; eauto.
-  now eapply invert_cumul_letin_l in c.
-Qed.
+  Lemma typing_spine_weaken_concl {cf:checker_flags} {Σ Γ T args S S'} : 
+    wf Σ.1 ->
+    typing_spine Σ Γ T args S ->
+    Σ ;;; Γ |- S <= S' ->
+    isType Σ Γ S' ->
+    typing_spine Σ Γ T args S'.
+  Proof.
+    intros wfΣ.  
+    induction 1 in S' => cum.
+    constructor; auto. now transitivity ty'.
+    intros isType.
+    econstructor; eauto.
+  Qed.
 
-Lemma typing_spine_letin {cf:checker_flags} {Σ Γ na b B T args S} : 
-  wf Σ.1 ->
-  typing_spine Σ Γ (T {0 := b}) args S ->
-  typing_spine Σ Γ (tLetIn na b B T) args S.
-Proof.
-  intros wfΣ Hsp.
-  depelim Hsp.
-  constructor. auto.
-  etransitivity. eapply red_cumul. eapply red1_red, red_zeta. auto.
-  econstructor; eauto.
-  etransitivity. eapply red_cumul. eapply red1_red, red_zeta. auto.
-Qed.
+  Lemma typing_spine_prod {cf:checker_flags} {Σ Γ na b B T args S} : 
+    wf Σ.1 ->
+    typing_spine Σ Γ (T {0 := b}) args S ->
+    isType Σ Γ (tProd na B T) ->
+    Σ ;;; Γ |- b : B ->
+    typing_spine Σ Γ (tProd na B T) (b :: args) S.
+  Proof.
+    intros wfΣ Hsp.
+    depelim Hsp.
+    econstructor; eauto. reflexivity.
+    constructor; auto with pcuic.
+    intros Har. eapply isType_tProd in Har as [? ?]; eauto using typing_wf_local.
+    intros Hb.
+    econstructor. 3:eauto. 2:reflexivity.
+    destruct i1 as [s Hs], i0 as [s' Hs'].
+    eexists. eapply type_Prod; eauto.
+    econstructor; eauto.
+  Qed.
 
-Lemma typing_spine_weaken_concl {cf:checker_flags} {Σ Γ T args S S'} : 
-  wf Σ.1 ->
-  typing_spine Σ Γ T args S ->
-  Σ ;;; Γ |- S <= S' ->
-  isType Σ Γ S' ->
-  typing_spine Σ Γ T args S'.
-Proof.
-  intros wfΣ.  
-  induction 1 in S' => cum.
-  constructor; auto. now transitivity ty'.
-  intros isType.
-  econstructor; eauto.
-Qed.
+  Lemma typing_spine_WAT_concl {cf:checker_flags} {Σ Γ T args S} : 
+    typing_spine Σ Γ T args S ->
+    isType Σ Γ S.
+  Proof.
+    induction 1; auto.
+  Qed.
 
-Lemma typing_spine_prod {cf:checker_flags} {Σ Γ na b B T args S} : 
-  wf Σ.1 ->
-  typing_spine Σ Γ (T {0 := b}) args S ->
-  isType Σ Γ (tProd na B T) ->
-  Σ ;;; Γ |- b : B ->
-  typing_spine Σ Γ (tProd na B T) (b :: args) S.
-Proof.
-  intros wfΣ Hsp.
-  depelim Hsp.
-  econstructor; eauto. reflexivity.
-  constructor; auto with pcuic.
-  intros Har. eapply isType_tProd in Har as [? ?]; eauto using typing_wf_local.
-  intros Hb.
-  econstructor. 3:eauto. 2:reflexivity.
-  destruct i1 as [s Hs], i0 as [s' Hs'].
-  eexists. eapply type_Prod; eauto.
-  econstructor; eauto.
-Qed.
+  Lemma type_mkProd_or_LetIn {cf:checker_flags} Σ Γ d u t s : 
+    wf Σ.1 ->
+    Σ ;;; Γ |- decl_type d : tSort u ->
+    Σ ;;; Γ ,, d |- t : tSort s ->
+    match decl_body d return Type with 
+    | Some b => Σ ;;; Γ |- mkProd_or_LetIn d t : tSort s
+    | None => Σ ;;; Γ |- mkProd_or_LetIn d t : tSort (Universe.sort_of_product u s)
+    end.
+  Proof.
+    intros wfΣ. destruct d as [na [b|] dty] => [Hd Ht|Hd Ht]; rewrite /mkProd_or_LetIn /=.
+    - have wf := typing_wf_local Ht.
+      depelim wf. clear l.
+      eapply type_Cumul. econstructor; eauto.
+      econstructor; eauto. now eapply typing_wf_universe in Ht.
+      transitivity (tSort s).
+      eapply red_cumul. eapply red1_red. constructor. reflexivity.
+    - have wf := typing_wf_local Ht.
+      depelim wf; clear l.
+      eapply type_Prod; eauto.
+  Qed.
 
-Lemma typing_spine_WAT_concl {cf:checker_flags} {Σ Γ T args S} : 
-  typing_spine Σ Γ T args S ->
-  isType Σ Γ S.
-Proof.
-  induction 1; auto.
-Qed.
+  Lemma type_it_mkProd_or_LetIn {cf:checker_flags} Σ Γ Γ' u t s : 
+    wf Σ.1 ->
+    wf_universe Σ u ->
+    type_local_ctx (lift_typing typing) Σ Γ Γ' u ->
+    Σ ;;; Γ ,,, Γ' |- t : tSort s ->
+    Σ ;;; Γ |- it_mkProd_or_LetIn Γ' t : tSort (Universe.sort_of_product u s).
+  Proof.
+    revert Γ u s t.
+    induction Γ'; simpl; auto; move=> Γ u s t wfΣ wfu equ Ht.
+    - eapply type_Cumul; eauto.
+      econstructor; eauto using typing_wf_local with pcuic.
+      eapply typing_wf_universe in Ht; auto with pcuic.
+      constructor. constructor.
+      eapply leq_universe_product.
+    - specialize (IHΓ' Γ  u (Universe.sort_of_product u s)); auto.
+      unfold app_context in Ht.
+      eapply type_Cumul.
+      eapply IHΓ'; auto.
+      destruct a as [na [b|] ty]; intuition auto.
+      destruct a as [na [b|] ty]; intuition auto.
+      { apply typing_wf_local in Ht as XX. inversion XX; subst.
+        eapply (type_mkProd_or_LetIn _ _ {| decl_body := Some b |}); auto.
+        + simpl. exact X0.π2.
+        + eapply type_Cumul; eauto.
+          econstructor; eauto with pcuic.
+          constructor. constructor. eapply leq_universe_product. }
+      eapply (type_mkProd_or_LetIn _ _ {| decl_body := None |}) => /=; eauto.
+      econstructor; eauto with pcuic.
+      eapply typing_wf_local in Ht.
+      depelim Ht; eapply All_local_env_app_inv in Ht; intuition auto.
+      now rewrite sort_of_product_twice.
+  Qed.
 
-Lemma type_mkProd_or_LetIn {cf:checker_flags} Σ Γ d u t s : 
-  wf Σ.1 ->
-  Σ ;;; Γ |- decl_type d : tSort u ->
-  Σ ;;; Γ ,, d |- t : tSort s ->
-  match decl_body d return Type with 
-  | Some b => Σ ;;; Γ |- mkProd_or_LetIn d t : tSort s
-  | None => Σ ;;; Γ |- mkProd_or_LetIn d t : tSort (Universe.sort_of_product u s)
-  end.
-Proof.
-  intros wfΣ. destruct d as [na [b|] dty] => [Hd Ht|Hd Ht]; rewrite /mkProd_or_LetIn /=.
-  - have wf := typing_wf_local Ht.
-    depelim wf. clear l.
-    eapply type_Cumul. econstructor; eauto.
-    econstructor; eauto. now eapply typing_wf_universe in Ht.
-    transitivity (tSort s).
-    eapply red_cumul. eapply red1_red. constructor. reflexivity.
-  - have wf := typing_wf_local Ht.
-    depelim wf; clear l.
-    eapply type_Prod; eauto.
-Qed.
+  Fixpoint sort_of_products us s :=
+    match us with
+    | [] => s
+    | u :: us => sort_of_products us (Universe.sort_of_product u s)
+    end.
 
-Lemma type_it_mkProd_or_LetIn {cf:checker_flags} Σ Γ Γ' u t s : 
-  wf Σ.1 ->
-  wf_universe Σ u ->
-  type_local_ctx (lift_typing typing) Σ Γ Γ' u ->
-  Σ ;;; Γ ,,, Γ' |- t : tSort s ->
-  Σ ;;; Γ |- it_mkProd_or_LetIn Γ' t : tSort (Universe.sort_of_product u s).
-Proof.
-  revert Γ u s t.
-  induction Γ'; simpl; auto; move=> Γ u s t wfΣ wfu equ Ht.
-  - eapply type_Cumul; eauto.
-    econstructor; eauto using typing_wf_local with pcuic.
-    eapply typing_wf_universe in Ht; auto with pcuic.
-    constructor. constructor.
-    eapply leq_universe_product.
-  - specialize (IHΓ' Γ  u (Universe.sort_of_product u s)); auto.
-    unfold app_context in Ht.
-    eapply type_Cumul.
-    eapply IHΓ'; auto.
-    destruct a as [na [b|] ty]; intuition auto.
-    destruct a as [na [b|] ty]; intuition auto.
-    { apply typing_wf_local in Ht as XX. inversion XX; subst.
-      eapply (type_mkProd_or_LetIn _ _ {| decl_body := Some b |}); auto.
-      + simpl. exact X0.π2.
-      + eapply type_Cumul; eauto.
-        econstructor; eauto with pcuic.
-        constructor. constructor. eapply leq_universe_product. }
-    eapply (type_mkProd_or_LetIn _ _ {| decl_body := None |}) => /=; eauto.
-    econstructor; eauto with pcuic.
-    eapply typing_wf_local in Ht.
-    depelim Ht; eapply All_local_env_app_inv in Ht; intuition auto.
-    now rewrite sort_of_product_twice.
-Qed.
+  Lemma leq_universe_sort_of_products_mon {cf} Σ u u' v v' : 
+    Forall2 (leq_universe Σ) u u' ->
+    leq_universe Σ v v' ->
+    leq_universe Σ (sort_of_products u v) (sort_of_products u' v').
+  Proof.
+    intros hu; induction hu in v, v' |- *; simpl; auto with pcuic.
+    intros lev. eapply IHhu.
+    eapply leq_universe_product_mon => //.
+  Qed.
 
-Fixpoint sort_of_products us s :=
-  match us with
-  | [] => s
-  | u :: us => sort_of_products us (Universe.sort_of_product u s)
-  end.
+  Lemma type_it_mkProd_or_LetIn_sorts {cf:checker_flags} Σ Γ Γ' us t s : 
+    wf Σ.1 ->
+    sorts_local_ctx (lift_typing typing) Σ Γ Γ' us ->
+    Σ ;;; Γ ,,, Γ' |- t : tSort s ->
+    Σ ;;; Γ |- it_mkProd_or_LetIn Γ' t : tSort (sort_of_products us s).
+  Proof.
+    revert Γ us s t.
+    induction Γ'; simpl; auto; move=> Γ us s t wfΣ equ Ht.
+    - destruct us => //.
+    - destruct a as [na [b|] ty]; intuition auto.
+      * destruct a0 as [s' Hs].
+        eapply IHΓ'; eauto.
+        eapply (type_mkProd_or_LetIn _ _ {| decl_body := Some b |}); auto.
+        simpl. exact Hs.
+      * destruct us => //. destruct equ.
+        simpl.   
+        eapply IHΓ'; eauto.
+        apply (type_mkProd_or_LetIn _ _ {| decl_body := None |}) => /=; eauto.
+  Qed.
 
-Lemma leq_universe_sort_of_products_mon {cf} Σ u u' v v' : 
-  Forall2 (leq_universe Σ) u u' ->
-  leq_universe Σ v v' ->
-  leq_universe Σ (sort_of_products u v) (sort_of_products u' v').
-Proof.
-  intros hu; induction hu in v, v' |- *; simpl; auto with pcuic.
-  intros lev. eapply IHhu.
-  eapply leq_universe_product_mon => //.
-Qed.
+  Lemma app_context_push Γ Δ Δ' d : (Γ ,,, Δ ,,, Δ') ,, d = (Γ ,,, Δ ,,, (Δ' ,, d)).
+  Proof.
+    reflexivity.
+  Qed.
 
-Lemma type_it_mkProd_or_LetIn_sorts {cf:checker_flags} Σ Γ Γ' us t s : 
-  wf Σ.1 ->
-  sorts_local_ctx (lift_typing typing) Σ Γ Γ' us ->
-  Σ ;;; Γ ,,, Γ' |- t : tSort s ->
-  Σ ;;; Γ |- it_mkProd_or_LetIn Γ' t : tSort (sort_of_products us s).
-Proof.
-  revert Γ us s t.
-  induction Γ'; simpl; auto; move=> Γ us s t wfΣ equ Ht.
-  - destruct us => //.
-  - destruct a as [na [b|] ty]; intuition auto.
-    * destruct a0 as [s' Hs].
-      eapply IHΓ'; eauto.
-      eapply (type_mkProd_or_LetIn _ _ {| decl_body := Some b |}); auto.
-      simpl. exact Hs.
-    * destruct us => //. destruct equ.
-      simpl.   
-      eapply IHΓ'; eauto.
-      apply (type_mkProd_or_LetIn _ _ {| decl_body := None |}) => /=; eauto.
-Qed.
-
-Lemma app_context_push Γ Δ Δ' d : (Γ ,,, Δ ,,, Δ') ,, d = (Γ ,,, Δ ,,, (Δ' ,, d)).
-Proof.
-  reflexivity.
-Qed.
-
-Hint Extern 4 (_ ;;; _ |- _ <= _) => reflexivity : pcuic.
-Ltac pcuic := eauto 5 with pcuic.
+  Hint Extern 4 (_ ;;; _ |- _ <= _) => reflexivity : pcuic.
+  Ltac pcuic := eauto 5 with pcuic.
 
 
-Lemma subslet_app_closed {cf:checker_flags} Σ Γ s s' Δ Δ' : 
-  subslet Σ Γ s Δ ->
-  subslet Σ Γ s' Δ' ->
-  closed_ctx Δ ->
-  subslet Σ Γ (s ++ s') (Δ' ,,, Δ).
-Proof.
-  induction 1 in s', Δ'; simpl; auto; move=> sub' => /andb_and [clctx clt];
-  try constructor; auto.
-  - pose proof (subslet_length X). rewrite Nat.add_0_r in clt.
-    rewrite /= -H in clt.
-    rewrite subst_app_simpl /= (subst_closedn s') //.
-  - pose proof (subslet_length X). rewrite Nat.add_0_r in clt.
-    rewrite /= -H in clt. move/andb_and: clt => [clt clT].
-    replace (subst0 s t) with (subst0 (s ++ s') t).
-    + constructor; auto.
-      rewrite !subst_app_simpl /= !(subst_closedn s') //.
-    + rewrite !subst_app_simpl /= !(subst_closedn s') //.
-Qed.
+  Lemma subslet_app_closed {cf:checker_flags} Σ Γ s s' Δ Δ' : 
+    subslet Σ Γ s Δ ->
+    subslet Σ Γ s' Δ' ->
+    closed_ctx Δ ->
+    subslet Σ Γ (s ++ s') (Δ' ,,, Δ).
+  Proof.
+    induction 1 in s', Δ'; simpl; auto; move=> sub' => /andb_and [clctx clt];
+    try constructor; auto.
+    - pose proof (subslet_length X). rewrite Nat.add_0_r in clt.
+      rewrite /= -H in clt.
+      rewrite subst_app_simpl /= (subst_closedn s') //.
+    - pose proof (subslet_length X). rewrite Nat.add_0_r in clt.
+      rewrite /= -H in clt. move/andb_and: clt => [clt clT].
+      replace (subst0 s t) with (subst0 (s ++ s') t).
+      + constructor; auto.
+        rewrite !subst_app_simpl /= !(subst_closedn s') //.
+      + rewrite !subst_app_simpl /= !(subst_closedn s') //.
+  Qed.
 
-Hint Constructors subslet : core pcuic.
+  Hint Constructors subslet : core pcuic.
 
-Lemma subslet_app_inv {cf:checker_flags} Σ Γ Δ Δ' s : 
-  subslet Σ Γ s (Δ ,,, Δ') ->
-  subslet Σ Γ (skipn #|Δ'| s) Δ * 
-  subslet Σ Γ (firstn #|Δ'| s) (subst_context (skipn #|Δ'| s) 0 Δ').
-Proof.
-  intros sub. split.
-  - induction Δ' in Δ, s, sub |- *; simpl; first by rewrite skipn_0.
-    depelim sub; rewrite skipn_S; auto.
-  - induction Δ' in Δ, s, sub |- *; simpl; first by constructor.
-    destruct s; depelim sub.
-    * rewrite subst_context_snoc. constructor; eauto.
-      rewrite skipn_S Nat.add_0_r /=.
-      assert(#|Δ'| = #|firstn #|Δ'| s|).
-      { pose proof (subslet_length sub).
-        rewrite app_context_length in H.
-        rewrite firstn_length_le; lia. }
-      rewrite {3}H.
-      rewrite -subst_app_simpl.
-      now rewrite firstn_skipn.
-    * rewrite subst_context_snoc.
-      rewrite skipn_S Nat.add_0_r /=.
-      rewrite /subst_decl /map_decl /=.
-      specialize (IHΔ' _ _ sub).
-      epose proof (cons_let_def _ _ _ _ _ (subst (skipn #|Δ'| s0) #|Δ'| t0) 
-      (subst (skipn #|Δ'| s0) #|Δ'| T) IHΔ').
-      assert(#|Δ'| = #|firstn #|Δ'| s0|).
-      { pose proof (subslet_length sub).
-        rewrite app_context_length in H.
-        rewrite firstn_length_le; lia. }      
-      rewrite {3 6}H in X.
-      rewrite - !subst_app_simpl in X.
-      rewrite !firstn_skipn in X.
-      specialize (X t1).
-      rewrite {3}H in X.
-      now rewrite - !subst_app_simpl firstn_skipn in X.
-Qed.
+  Lemma subslet_app_inv {cf:checker_flags} Σ Γ Δ Δ' s : 
+    subslet Σ Γ s (Δ ,,, Δ') ->
+    subslet Σ Γ (skipn #|Δ'| s) Δ * 
+    subslet Σ Γ (firstn #|Δ'| s) (subst_context (skipn #|Δ'| s) 0 Δ').
+  Proof.
+    intros sub. split.
+    - induction Δ' in Δ, s, sub |- *; simpl; first by rewrite skipn_0.
+      depelim sub; rewrite skipn_S; auto.
+    - induction Δ' in Δ, s, sub |- *; simpl; first by constructor.
+      destruct s; depelim sub.
+      * rewrite subst_context_snoc. constructor; eauto.
+        rewrite skipn_S Nat.add_0_r /=.
+        assert(#|Δ'| = #|firstn #|Δ'| s|).
+        { pose proof (subslet_length sub).
+          rewrite app_context_length in H.
+          rewrite firstn_length_le; lia. }
+        rewrite {3}H.
+        rewrite -subst_app_simpl.
+        now rewrite firstn_skipn.
+      * rewrite subst_context_snoc.
+        rewrite skipn_S Nat.add_0_r /=.
+        rewrite /subst_decl /map_decl /=.
+        specialize (IHΔ' _ _ sub).
+        epose proof (cons_let_def _ _ _ _ _ (subst (skipn #|Δ'| s0) #|Δ'| t0) 
+        (subst (skipn #|Δ'| s0) #|Δ'| T) IHΔ').
+        assert(#|Δ'| = #|firstn #|Δ'| s0|).
+        { pose proof (subslet_length sub).
+          rewrite app_context_length in H.
+          rewrite firstn_length_le; lia. }      
+        rewrite {3 6}H in X.
+        rewrite - !subst_app_simpl in X.
+        rewrite !firstn_skipn in X.
+        specialize (X t1).
+        rewrite {3}H in X.
+        now rewrite - !subst_app_simpl firstn_skipn in X.
+  Qed.
 
-Lemma subslet_inds_gen {cf:checker_flags} Σ ind mdecl idecl :
-  wf Σ ->
-  declared_inductive Σ ind mdecl idecl ->
-  let u := PCUICLookup.abstract_instance (ind_universes mdecl) in
-  subslet (Σ, ind_universes mdecl) [] (inds (inductive_mind ind) u (ind_bodies mdecl))
-    (arities_context (ind_bodies mdecl)).
-Proof.
-  intros wfΣ isdecl u.
-  unfold inds.
-  pose proof (proj1 isdecl) as declm'. 
-  apply PCUICWeakeningEnv.on_declared_minductive in declm' as [oind oc]; auto.
-  clear oc.
-  assert (Alli (fun i x =>
-   (Σ, ind_universes mdecl) ;;; [] |- tInd {| inductive_mind := inductive_mind ind; inductive_ind := i |} u : (ind_type x)) 0 (ind_bodies mdecl)).
-  { apply forall_nth_error_Alli. intros.
-    eapply Alli_nth_error in oind; eauto. simpl in oind.
-    destruct oind. destruct onArity as [s Hs].
-    eapply type_Cumul; eauto.
-    econstructor; eauto. split; eauto with pcuic.
-    eapply consistent_instance_ext_abstract_instance; eauto.
-    eapply declared_inductive_wf_global_ext; eauto with pcuic.
-    rewrite (subst_instance_ind_type_id Σ _ {| inductive_mind := inductive_mind ind; inductive_ind := i |}); eauto.
-    destruct isdecl. split; eauto. reflexivity. }
-  clear oind.
-  revert X. clear onNpars.
-  generalize (le_n #|ind_bodies mdecl|).
-  generalize (ind_bodies mdecl) at 1 3 4 5.
-  induction l using rev_ind; simpl; first constructor.
-  rewrite /subst_instance /= /map_context.
-  simpl. rewrite /arities_context rev_map_spec /=.
-  rewrite map_app /= rev_app_distr /=. 
-  rewrite /= app_length /= Nat.add_1_r.
-  constructor.
-  - rewrite -rev_map_spec. apply IHl; try lia.
-    eapply Alli_app in X; intuition auto.
-  - eapply Alli_app in X as [oind Hx].
-    depelim Hx. clear Hx.
-    rewrite Nat.add_0_r in t.
-    rewrite subst_closedn; auto. 
-    + eapply typecheck_closed in t as [? ?]; auto.
-      destruct p as [? ?].
-      now move/andb_and: i0=> [? ?].
-Qed.
+  Lemma subslet_inds_gen {cf:checker_flags} Σ ind mdecl idecl :
+    wf Σ ->
+    declared_inductive Σ ind mdecl idecl ->
+    let u := PCUICLookup.abstract_instance (ind_universes mdecl) in
+    subslet (Σ, ind_universes mdecl) [] (inds (inductive_mind ind) u (ind_bodies mdecl))
+      (arities_context (ind_bodies mdecl)).
+  Proof.
+    intros wfΣ isdecl u.
+    unfold inds.
+    pose proof (proj1 isdecl) as declm'. 
+    apply PCUICWeakeningEnv.on_declared_minductive in declm' as [oind oc]; auto.
+    clear oc.
+    assert (Alli (fun i x =>
+    (Σ, ind_universes mdecl) ;;; [] |- tInd {| inductive_mind := inductive_mind ind; inductive_ind := i |} u : (ind_type x)) 0 (ind_bodies mdecl)).
+    { apply forall_nth_error_Alli. intros.
+      eapply Alli_nth_error in oind; eauto. simpl in oind.
+      destruct oind. destruct onArity as [s Hs].
+      eapply type_Cumul; eauto.
+      econstructor; eauto. split; eauto with pcuic.
+      eapply consistent_instance_ext_abstract_instance; eauto.
+      eapply declared_inductive_wf_global_ext; eauto with pcuic.
+      rewrite (subst_instance_ind_type_id Σ _ {| inductive_mind := inductive_mind ind; inductive_ind := i |}); eauto.
+      destruct isdecl. split; eauto. reflexivity. }
+    clear oind.
+    revert X. clear onNpars.
+    generalize (le_n #|ind_bodies mdecl|).
+    generalize (ind_bodies mdecl) at 1 3 4 5.
+    induction l using rev_ind; simpl; first constructor.
+    rewrite /subst_instance /= /map_context.
+    simpl. rewrite /arities_context rev_map_spec /=.
+    rewrite map_app /= rev_app_distr /=. 
+    rewrite /= app_length /= Nat.add_1_r.
+    constructor.
+    - rewrite -rev_map_spec. apply IHl; try lia.
+      eapply Alli_app in X; intuition auto.
+    - eapply Alli_app in X as [oind Hx].
+      depelim Hx. clear Hx.
+      rewrite Nat.add_0_r in t.
+      rewrite subst_closedn; auto. 
+      + eapply typecheck_closed in t as [? ?]; auto.
+        destruct p as [? ?].
+        now move/andb_and: i0=> [? ?].
+  Qed.
 
-Lemma subslet_inds {cf:checker_flags} Σ ind u mdecl idecl :
-  wf Σ.1 ->
-  declared_inductive Σ.1 ind mdecl idecl ->
-  consistent_instance_ext Σ (ind_universes mdecl) u ->
-  subslet Σ [] (inds (inductive_mind ind) u (ind_bodies mdecl))
-    (subst_instance u (arities_context (ind_bodies mdecl))).
-Proof.
-  intros wfΣ isdecl univs.
-  unfold inds.
-  pose proof (proj1 isdecl) as declm.
-  apply PCUICWeakeningEnv.on_declared_minductive in declm as [oind oc]; auto.
-  clear oc.
-  assert (Alli (fun i x => 
-    Σ ;;; [] |- tInd {| inductive_mind := inductive_mind ind; inductive_ind := i |} u : subst_instance u (ind_type x)) 0 (ind_bodies mdecl)). 
-  { apply forall_nth_error_Alli.
-    econstructor; eauto. split; eauto. simpl. eapply isdecl. }
-  clear oind.
-  revert X. clear onNpars.
-  generalize (le_n #|ind_bodies mdecl|).
-  generalize (ind_bodies mdecl) at 1 3 4 5.
-  induction l using rev_ind; simpl; first constructor.
-  rewrite /subst_instance /= /map_context.
-  simpl. rewrite /arities_context rev_map_spec /=.
-  rewrite map_app /= rev_app_distr /=. 
-  rewrite {1}/map_decl /= app_length /= Nat.add_1_r.
-  constructor.
-  - rewrite -rev_map_spec. apply IHl; try lia.
-    eapply Alli_app in X; intuition auto.
-  - eapply Alli_app in X as [oind Hx].
-    depelim Hx. clear Hx.
-    rewrite Nat.add_0_r in t.
-    rewrite subst_closedn; auto.
-    + now eapply type_closed in t.
-Qed.
+  Lemma subslet_inds {cf:checker_flags} Σ ind u mdecl idecl :
+    wf Σ.1 ->
+    declared_inductive Σ.1 ind mdecl idecl ->
+    consistent_instance_ext Σ (ind_universes mdecl) u ->
+    subslet Σ [] (inds (inductive_mind ind) u (ind_bodies mdecl))
+      (subst_instance u (arities_context (ind_bodies mdecl))).
+  Proof.
+    intros wfΣ isdecl univs.
+    unfold inds.
+    pose proof (proj1 isdecl) as declm.
+    apply PCUICWeakeningEnv.on_declared_minductive in declm as [oind oc]; auto.
+    clear oc.
+    assert (Alli (fun i x => 
+      Σ ;;; [] |- tInd {| inductive_mind := inductive_mind ind; inductive_ind := i |} u : subst_instance u (ind_type x)) 0 (ind_bodies mdecl)). 
+    { apply forall_nth_error_Alli.
+      econstructor; eauto. split; eauto. simpl. eapply isdecl. }
+    clear oind.
+    revert X. clear onNpars.
+    generalize (le_n #|ind_bodies mdecl|).
+    generalize (ind_bodies mdecl) at 1 3 4 5.
+    induction l using rev_ind; simpl; first constructor.
+    rewrite /subst_instance /= /map_context.
+    simpl. rewrite /arities_context rev_map_spec /=.
+    rewrite map_app /= rev_app_distr /=. 
+    rewrite {1}/map_decl /= app_length /= Nat.add_1_r.
+    constructor.
+    - rewrite -rev_map_spec. apply IHl; try lia.
+      eapply Alli_app in X; intuition auto.
+    - eapply Alli_app in X as [oind Hx].
+      depelim Hx. clear Hx.
+      rewrite Nat.add_0_r in t.
+      rewrite subst_closedn; auto.
+      + now eapply type_closed in t.
+  Qed.
 
-Lemma weaken_subslet {cf:checker_flags} Σ s Δ Γ :
-  wf Σ.1 ->
-  wf_local Σ Γ -> 
-  subslet Σ [] s Δ -> subslet Σ Γ s Δ.
-Proof.
-  intros wfΣ wfΔ.
-  induction 1; constructor; auto.
-  + eapply (weaken_ctx (Γ:=[]) Γ); eauto.
-  + eapply (weaken_ctx (Γ:=[]) Γ); eauto.
-Qed.
+  Lemma weaken_subslet {cf:checker_flags} Σ s Δ Γ :
+    wf Σ.1 ->
+    wf_local Σ Γ -> 
+    subslet Σ [] s Δ -> subslet Σ Γ s Δ.
+  Proof.
+    intros wfΣ wfΔ.
+    induction 1; constructor; auto.
+    + eapply (weaken_ctx (Γ:=[]) Γ); eauto.
+    + eapply (weaken_ctx (Γ:=[]) Γ); eauto.
+  Qed.
 
 
 
-Set Default Goal Selector "1".
+  Set Default Goal Selector "1".
 
-Lemma isType_substitution_it_mkProd_or_LetIn {cf:checker_flags} {Σ Γ Δ T s} : 
-  wf Σ.1 ->
-  subslet Σ Γ s Δ ->
-  isType Σ Γ (it_mkProd_or_LetIn Δ T) ->
-  isType Σ Γ (subst0 s T).
-Proof.
-  intros wfΣ sub [s' Hs].
-  exists s'.
-  revert Γ s sub Hs. 
-  generalize (le_n #|Δ|).
-  generalize #|Δ| at 2.
-  induction n in Δ, T |- *.
-  - destruct Δ; simpl; intros; try (elimtype False; lia).
-    depelim sub.
-    rewrite subst_empty; auto.
-  - destruct Δ using rev_ind; try clear IHΔ.
-    + intros Hn Γ s sub; now depelim sub; rewrite subst_empty.
-    + rewrite app_length Nat.add_1_r /= => Hn Γ s sub.
-    pose proof (subslet_length sub). rewrite app_length /= Nat.add_1_r in H.
-    have Hl : #|l| = #|firstn #|l| s|.
-    { rewrite firstn_length_le; lia. }
-    destruct x as [na [b|] ty] => /=;
-    rewrite it_mkProd_or_LetIn_app /= /mkProd_or_LetIn /=.
-    
-    intros Hs.
-    assert (wfs' := typing_wf_universe wfΣ Hs).
-    eapply inversion_LetIn in Hs as [? [? [? [? [? ?]]]]]; auto.
-    eapply substitution_let in t1; auto.
-    eapply invert_cumul_letin_l in c; auto.
-    pose proof (subslet_app_inv _ _ _ _ _ sub) as [subl subr].
-    depelim subl. depelim subl. rewrite subst_empty in H0. rewrite H0 in subr.
-    specialize (IHn (subst_context [b] 0 l) (subst [b] #|l| T) ltac:(rewrite subst_context_length; lia)).
-    specialize (IHn _ _ subr).
-    rewrite /subst1 subst_it_mkProd_or_LetIn Nat.add_0_r in t1.
-    rewrite !subst_empty in t3.
-    forward IHn.
-    eapply type_Cumul. eapply t1. econstructor; intuition eauto using typing_wf_local with pcuic.
-    eapply c. rewrite {2}Hl in IHn.
-    now rewrite -subst_app_simpl -H0 firstn_skipn in IHn.
-    
-    intros Hs.
-    assert (wfs' := typing_wf_universe wfΣ Hs).
-    eapply inversion_Prod in Hs as [? [? [? [? ?]]]]; auto.
-    pose proof (subslet_app_inv _ _ _ _ _ sub) as [subl subr].
-    depelim subl; depelim subl. rewrite subst_empty in t2. rewrite H0 in subr.
-    epose proof (substitution0 _ _ na _ _ _ _ wfΣ t0 t2).
-    specialize (IHn (subst_context [t1] 0 l) (subst [t1] #|l| T)).
-    forward IHn. rewrite subst_context_length; lia.
-    specialize (IHn _ _ subr).
-    rewrite /subst1 subst_it_mkProd_or_LetIn Nat.add_0_r in X.
-    forward IHn.
-    eapply type_Cumul. simpl in X. eapply X.
-    econstructor; eauto with pcuic.
-    eapply cumul_Sort_inv in c.
-    do 2 constructor.
-    transitivity (Universe.sort_of_product x x0).
-    eapply leq_universe_product. auto.
-    rewrite {2}Hl in IHn.
-    now rewrite -subst_app_simpl -H0 firstn_skipn in IHn.
-Qed.
+  Lemma isType_substitution_it_mkProd_or_LetIn {cf:checker_flags} {Σ Γ Δ T s} : 
+    wf Σ.1 ->
+    subslet Σ Γ s Δ ->
+    isType Σ Γ (it_mkProd_or_LetIn Δ T) ->
+    isType Σ Γ (subst0 s T).
+  Proof.
+    intros wfΣ sub [s' Hs].
+    exists s'.
+    revert Γ s sub Hs. 
+    generalize (le_n #|Δ|).
+    generalize #|Δ| at 2.
+    induction n in Δ, T |- *.
+    - destruct Δ; simpl; intros; try (elimtype False; lia).
+      depelim sub.
+      rewrite subst_empty; auto.
+    - destruct Δ using rev_ind; try clear IHΔ.
+      + intros Hn Γ s sub; now depelim sub; rewrite subst_empty.
+      + rewrite app_length Nat.add_1_r /= => Hn Γ s sub.
+      pose proof (subslet_length sub). rewrite app_length /= Nat.add_1_r in H.
+      have Hl : #|l| = #|firstn #|l| s|.
+      { rewrite firstn_length_le; lia. }
+      destruct x as [na [b|] ty] => /=;
+      rewrite it_mkProd_or_LetIn_app /= /mkProd_or_LetIn /=.
+      
+      intros Hs.
+      assert (wfs' := typing_wf_universe wfΣ Hs).
+      eapply inversion_LetIn in Hs as [? [? [? [? [? ?]]]]]; auto.
+      eapply substitution_let in t1; auto.
+      eapply equality_LetIn_l_inv in c; auto.
+      pose proof (subslet_app_inv _ _ _ _ _ sub) as [subl subr].
+      depelim subl. depelim subl. rewrite subst_empty in H0. rewrite H0 in subr.
+      specialize (IHn (subst_context [b] 0 l) (subst [b] #|l| T) ltac:(rewrite subst_context_length; lia)).
+      specialize (IHn _ _ subr).
+      rewrite /subst1 subst_it_mkProd_or_LetIn Nat.add_0_r in t1.
+      rewrite !subst_empty in t3.
+      forward IHn.
+      eapply type_Cumul. eapply t1. econstructor; intuition eauto using typing_wf_local with pcuic.
+      eapply c. rewrite {2}Hl in IHn.
+      now rewrite -subst_app_simpl -H0 firstn_skipn in IHn.
+      
+      intros Hs.
+      assert (wfs' := typing_wf_universe wfΣ Hs).
+      eapply inversion_Prod in Hs as [? [? [? [? ?]]]]; auto.
+      pose proof (subslet_app_inv _ _ _ _ _ sub) as [subl subr].
+      depelim subl; depelim subl. rewrite subst_empty in t2. rewrite H0 in subr.
+      epose proof (substitution0 _ _ na _ _ _ _ wfΣ t0 t2).
+      specialize (IHn (subst_context [t1] 0 l) (subst [t1] #|l| T)).
+      forward IHn. rewrite subst_context_length; lia.
+      specialize (IHn _ _ subr).
+      rewrite /subst1 subst_it_mkProd_or_LetIn Nat.add_0_r in X.
+      forward IHn.
+      eapply type_Cumul. simpl in X. eapply X.
+      econstructor; eauto with pcuic.
+      eapply cumul_Sort_inv in c.
+      do 2 constructor.
+      transitivity (Universe.sort_of_product x x0).
+      eapply leq_universe_product. auto.
+      rewrite {2}Hl in IHn.
+      now rewrite -subst_app_simpl -H0 firstn_skipn in IHn.
+  Qed.
 
-Lemma isType_tLetIn_red {cf:checker_flags} {Σ : global_env_ext} (HΣ' : wf Σ)
-      {Γ} (HΓ : wf_local Σ Γ) {na t A B}
-  : isType Σ Γ (tLetIn na t A B) -> isType Σ Γ (B {0:=t}).
-Proof.
-  intro HH.
-  destruct HH as [s H].
-  exists s.
-  assert (Hs := typing_wf_universe HΣ' H).
-  apply inversion_LetIn in H; tas. destruct H as [s1 [A' [HA [Ht [HB H]]]]].
-  eapply type_Cumul with (A' {0 := t}) _. eapply substitution_let in HB; eauto.
-  * econstructor; eauto with pcuic.
-  * eapply cumul_Sort_r_inv in H.
-    destruct H as [s' [H H']].
-    eapply cumul_trans with (tSort s'); eauto.
-    eapply red_cumul.
-    apply invert_red_letin in H as [H|H] => //.
-    destruct H as [d' [ty' [b' [[[reds ?] ?] ?]]]].
-    discriminate.
-    now repeat constructor.
-Qed.
+  Lemma isType_tLetIn_red {cf:checker_flags} {Σ : global_env_ext} (HΣ' : wf Σ)
+        {Γ} (HΓ : wf_local Σ Γ) {na t A B}
+    : isType Σ Γ (tLetIn na t A B) -> isType Σ Γ (B {0:=t}).
+  Proof.
+    intro HH.
+    destruct HH as [s H].
+    exists s.
+    assert (Hs := typing_wf_universe HΣ' H).
+    apply inversion_LetIn in H; tas. destruct H as [s1 [A' [HA [Ht [HB H]]]]].
+    eapply type_Cumul with (A' {0 := t}) _. eapply substitution_let in HB; eauto.
+    * econstructor; eauto with pcuic.
+    * eapply equality_Sort_r_inv in H.
+      destruct H as [s' [H H']].
+      eapply cumul_trans with (tSort s'); eauto.
+      eapply red_cumul.
+      apply invert_red_letin in H as [H|H] => //.
+      destruct H as [d' [ty' [b' [[[reds ?] ?] ?]]]].
+      discriminate.
+      now repeat constructor.
+  Qed.
 
-Lemma isType_tLetIn_dom {cf:checker_flags} {Σ : global_env_ext} (HΣ' : wf Σ)
-      {Γ} (HΓ : wf_local Σ Γ) {na t A B}
-  : isType Σ Γ (tLetIn na t A B) -> Σ ;;; Γ |- t : A.
-Proof.
-  intro HH.
-  destruct HH as [s H].
-  apply inversion_LetIn in H; tas. now destruct H as [s1 [A' [HA [Ht [HB H]]]]].
-Qed.
+  Lemma isType_tLetIn_dom {cf:checker_flags} {Σ : global_env_ext} (HΣ' : wf Σ)
+        {Γ} (HΓ : wf_local Σ Γ) {na t A B}
+    : isType Σ Γ (tLetIn na t A B) -> Σ ;;; Γ |- t : A.
+  Proof.
+    intro HH.
+    destruct HH as [s H].
+    apply inversion_LetIn in H; tas. now destruct H as [s1 [A' [HA [Ht [HB H]]]]].
+  Qed.
 
-Lemma on_minductive_wf_params {cf : checker_flags} {Σ : global_env_ext} {wfΣ : wf Σ} {ind mdecl} {u} :
-  declared_minductive Σ.1 ind mdecl ->
-  consistent_instance_ext Σ (ind_universes mdecl) u ->
-  wf_local Σ (subst_instance u (ind_params mdecl)).
-Proof.
-  intros; eapply (wf_local_instantiate _ (InductiveDecl mdecl)); eauto.
-  eapply on_declared_minductive in H; auto.
-  now apply onParams in H.
-Qed.
+  Lemma on_minductive_wf_params {cf : checker_flags} {Σ : global_env_ext} {wfΣ : wf Σ} {ind mdecl} {u} :
+    declared_minductive Σ.1 ind mdecl ->
+    consistent_instance_ext Σ (ind_universes mdecl) u ->
+    wf_local Σ (subst_instance u (ind_params mdecl)).
+  Proof.
+    intros; eapply (wf_local_instantiate _ (InductiveDecl mdecl)); eauto.
+    eapply on_declared_minductive in H; auto.
+    now apply onParams in H.
+  Qed.
 
-Lemma it_mkProd_or_LetIn_wf_local {cf:checker_flags} Σ Γ Δ T U : 
-  wf Σ.1 ->
-  Σ ;;; Γ |- it_mkProd_or_LetIn Δ T : U -> wf_local Σ (Γ ,,, Δ).
-Proof.
-  move=> wfΣ; move: Γ T U.
-  induction Δ using rev_ind => Γ T U.
-  + simpl. intros. now eapply typing_wf_local in X.
-  + rewrite it_mkProd_or_LetIn_app.
-    destruct x as [na [b|] ty]; cbn; move=> H.
-    * apply inversion_LetIn in H as (s1 & A & H0 & H1 & H2 & H3); auto.
-      eapply All_local_env_app; split; pcuic.
-      eapply All_local_env_app. split. repeat constructor. now exists s1.
-      auto. apply IHΔ in H2.
-      eapply All_local_env_app_inv in H2. intuition auto.
-      eapply All_local_env_impl; eauto. simpl. intros.
-      now rewrite app_context_assoc.
-    * apply inversion_Prod in H as (s1 & A & H0 & H1 & H2); auto.
-      eapply All_local_env_app; split; pcuic. 
-      eapply All_local_env_app. split. repeat constructor. now exists s1.
-      apply IHΔ in H1.
-      eapply All_local_env_app_inv in H1. intuition auto.
-      eapply All_local_env_impl; eauto. simpl. intros.
-      now rewrite app_context_assoc.
-Qed.
+  Lemma it_mkProd_or_LetIn_wf_local {cf:checker_flags} Σ Γ Δ T U : 
+    wf Σ.1 ->
+    Σ ;;; Γ |- it_mkProd_or_LetIn Δ T : U -> wf_local Σ (Γ ,,, Δ).
+  Proof.
+    move=> wfΣ; move: Γ T U.
+    induction Δ using rev_ind => Γ T U.
+    + simpl. intros. now eapply typing_wf_local in X.
+    + rewrite it_mkProd_or_LetIn_app.
+      destruct x as [na [b|] ty]; cbn; move=> H.
+      * apply inversion_LetIn in H as (s1 & A & H0 & H1 & H2 & H3); auto.
+        eapply All_local_env_app; split; pcuic.
+        eapply All_local_env_app. split. repeat constructor. now exists s1.
+        auto. apply IHΔ in H2.
+        eapply All_local_env_app_inv in H2. intuition auto.
+        eapply All_local_env_impl; eauto. simpl. intros.
+        now rewrite app_context_assoc.
+      * apply inversion_Prod in H as (s1 & A & H0 & H1 & H2); auto.
+        eapply All_local_env_app; split; pcuic. 
+        eapply All_local_env_app. split. repeat constructor. now exists s1.
+        apply IHΔ in H1.
+        eapply All_local_env_app_inv in H1. intuition auto.
+        eapply All_local_env_impl; eauto. simpl. intros.
+        now rewrite app_context_assoc.
+  Qed.
 
-Lemma isType_it_mkProd_or_LetIn_wf_local {cf:checker_flags} Σ Γ Δ T : 
-  wf Σ.1 ->
-  isType Σ Γ (it_mkProd_or_LetIn Δ T) -> wf_local Σ (Γ ,,, Δ).
-Proof.
-  move=> wfΣ [s Hs].
-  now eapply it_mkProd_or_LetIn_wf_local in Hs.
-Qed.
+  Lemma isType_it_mkProd_or_LetIn_wf_local {cf:checker_flags} Σ Γ Δ T : 
+    wf Σ.1 ->
+    isType Σ Γ (it_mkProd_or_LetIn Δ T) -> wf_local Σ (Γ ,,, Δ).
+  Proof.
+    move=> wfΣ [s Hs].
+    now eapply it_mkProd_or_LetIn_wf_local in Hs.
+  Qed.
 
-Lemma isType_weaken {cf:checker_flags} Σ Γ T :
-  wf Σ.1 -> wf_local Σ Γ ->
-  isType Σ [] T ->
-  isType Σ Γ T.
-Proof.
-  move=> wfΣ wfΓ [s hs].
-  exists s.
-  unshelve epose proof (subject_closed wfΣ hs); eauto.
-  eapply (weakening _ _ Γ) in hs => //.
-  rewrite lift_closed in hs => //.
-  now rewrite app_context_nil_l in hs.
-  now rewrite app_context_nil_l.
-Qed.
+  Lemma isType_weaken {cf:checker_flags} Σ Γ T :
+    wf Σ.1 -> wf_local Σ Γ ->
+    isType Σ [] T ->
+    isType Σ Γ T.
+  Proof.
+    move=> wfΣ wfΓ [s hs].
+    exists s.
+    unshelve epose proof (subject_closed wfΣ hs); eauto.
+    eapply (weakening _ _ Γ) in hs => //.
+    rewrite lift_closed in hs => //.
+    now rewrite app_context_nil_l in hs.
+    now rewrite app_context_nil_l.
+  Qed.
 
-Lemma subst_telescope_subst_instance u s k Γ :
-  subst_telescope (map (subst_instance u) s) k 
-    (subst_instance u Γ) =
-  subst_instance u (subst_telescope s k Γ).
-Proof.
-  rewrite /subst_telescope /subst_instance /= /subst_instance_context /map_context.
-  rewrite map_mapi mapi_map. apply mapi_ext.
-  intros. rewrite !compose_map_decl; apply map_decl_ext => ?.
-  now rewrite -subst_instance_subst.
-Qed.
+  Lemma subst_telescope_subst_instance u s k Γ :
+    subst_telescope (map (subst_instance u) s) k 
+      (subst_instance u Γ) =
+    subst_instance u (subst_telescope s k Γ).
+  Proof.
+    rewrite /subst_telescope /subst_instance /= /subst_instance_context /map_context.
+    rewrite map_mapi mapi_map. apply mapi_ext.
+    intros. rewrite !compose_map_decl; apply map_decl_ext => ?.
+    now rewrite -subst_instance_subst.
+  Qed.
+End WfEnv.
